Remove requirement that tags are [handlerTag] in [tim_intro].
Fixed up Delphine's proofs, so hopefully this is not a problem.  If
it is a problem, then there is another route to go, which seems true
of the current definitions: the alternative is to make manifest in
the [handler_correct] premises that the initial memory has contents
with tags equal to [handlerTag].  This is true because [build_cache]
sets up the memory that way.

ifc-machine/pico/tmu/cmach/Concrete.v
@@ -108,7 +108,7 @@ End WithListNotations.
 
 (** Cache spec when reading from, writing to *)
 Inductive tag_in_mem (m: list (@Atom Z)) addr tagv : Prop := 
-| tim_intro : index_list_Z addr m = Some (tagv,handlerTag) ->
+| tim_intro : forall tag, index_list_Z addr m = Some (tagv,tag) ->
               tag_in_mem m addr tagv.
 
 (* Tests the cache line *)  
